checker/coq/element.v
@@ -155,3 +155,167 @@ Proof.
 Qed.
 
 Definition ElementSolCheck := mkSolChecker ElemConstraint eval_element_sol eval_element_sol_valid.
+
+
+(* Now add member/nonmember constraints *)
+Inductive member : Type :=
+| Mem : iterm -> list iterm -> member.
+
+Ltac list_ext :=
+  repeat (
+  match goal with
+    | [ |- context[List.Exists _ _] ] => rewrite List.Exists_exists
+    | [ |- context[List.Forall _ _] ] => rewrite List.Forall_forall                                 
+    | [ |- context[List.forallb _ _ = true] ] => rewrite List.forallb_forall
+    | [ |- context[List.existsb _ _ = true] ] => rewrite List.existsb_exists
+    | [ H : context[ List.Exists _ _ ] |- _ ] => rewrite List.Exists_exists in H
+    | [ H : context[List.Forall _ _] |- _ ] => rewrite List.Forall_forall in H
+    | [ H : context[List.forallb _ _ = true] |- _ ] => rewrite List.forallb_forall in H
+    | [ H : context[List.existsb _ _ = true] |- _ ] => rewrite List.existsb_exists in H
+  end).
+
+Definition eval_member mem theta :=
+  match mem with
+      | Mem z xs => List.Exists (fun x => (eval_iterm z theta) = (eval_iterm x theta)) xs
+  end.
+Definition check_member_sol mem theta :=
+  match mem with
+    | Mem z xs =>
+      let z' := eval_iterm z theta in
+      List.existsb (fun x => Z.eqb z' (eval_iterm x theta)) xs
+  end.
+Lemma check_member_sol_valid : forall mem theta, check_member_sol mem theta = true -> eval_member mem theta.
+Proof.
+  intros mem theta; destruct mem as [z xs].
+  unfold check_member_sol, eval_member.
+  list_ext; tsimpl; elim H; clear H; intros x Hx; exists x.
+  now rewrite Z.eqb_eq in Hx.
+Qed.
+Definition check_member_unsat mem ds :=
+  match mem with
+    | Mem z xs =>
+      let z' := term_dom ds z in
+      List.forallb (fun x => dom_unsatb (dom_meet z' (term_dom ds x))) xs
+  end.
+Lemma check_member_unsat_valid :
+  forall mem ds, check_member_unsat mem ds = true -> forall theta, eval_domset ds theta -> ~ eval_member mem theta.
+Proof.
+  intros mem ds; unfold check_member_unsat, eval_member; destruct mem as [z xs].
+  list_ext; dom_simpl.
+  intros Hf theta Hds. intro Hex.
+  list_ext; elim Hex; clear Hex; intros x Hex; destruct Hex as [Hin Hx].
+  specialize (Hf x Hin).
+  rewrite dom_unsatb_unsat in Hf; unfold dom_unsat in Hf; specialize (Hf (eval_iterm x theta)).
+  rewrite dom_meet_iff in Hf.
+  assert (sat_dom (term_dom ds z) (eval_iterm x theta) /\ sat_dom (term_dom ds x) (eval_iterm x theta)).
+    split; [rewrite <- Hx; apply term_dom_valid | apply term_dom_valid]; assumption.
+  contradiction.
+Qed.
+
+Inductive notmember : Type :=
+  | Notmem : iterm -> list iterm -> notmember.
+
+Definition eval_notmember nmem theta :=
+  match nmem with
+    | Notmem z xs => List.Forall (fun x => (eval_iterm z theta) <> (eval_iterm x theta)) xs
+  end.
+Definition check_notmem_sol nmem theta :=
+  match nmem with
+    | Notmem z xs =>
+      let z' := eval_iterm z theta in
+      List.forallb (fun x => negb (Z.eqb z' (eval_iterm x theta))) xs
+  end.
+Lemma check_notmem_sol_valid : forall nmem theta, check_notmem_sol nmem theta = true -> eval_notmember nmem theta.
+Proof.
+  intros nmem theta; destruct nmem as [z xs]; unfold check_notmem_sol, eval_notmember.
+  list_ext.
+  intros Hc x Hin; specialize (Hc x Hin).
+  tsimpl.
+  rewrite <- Z.eqb_eq in H; congruence.
+Qed.
+
+Fixpoint notmem_holes ds xs holes :=
+  match xs with
+    | nil => holes
+    | cons x xs' =>
+      match db_constant_value (range_of_dom (term_dom ds x)) with
+        | None => notmem_holes ds xs' holes
+        | Some k => notmem_holes ds xs' (zset.add holes k)
+      end
+  end.
+Lemma notmem_holes_holes :
+  forall ds theta, eval_domset ds theta ->
+                   forall xs holes k, ~ zset.mem holes k -> List.Forall (fun x => eval_iterm x theta <> k) xs -> ~ zset.mem (notmem_holes ds xs holes) k.
+Proof.
+  intros ds theta Hds xs holes k Hnm Hf.
+  generalize holes Hnm; clear Hnm holes.
+  induction xs.
+  + intros; trivial.
+  + intros holes Hnm.
+    unfold notmem_holes; fold notmem_holes.
+    eqelim (db_constant_value (range_of_dom (term_dom ds a))).
+    - assert (Ha := db_constant_value_2 (range_of_dom (term_dom ds a)) z H0).
+      list_ext.
+      assert (forall x, List.In x xs -> eval_iterm x theta <> k) as H'.
+        intros x Hin; apply Hf; now apply List.in_cons.
+      apply (IHxs H' (zset.add holes z)).
+      intro Hmem; apply zset.mem_addk_if in Hmem.
+      destruct Hmem as [Hmem | Hmem]; try contradiction.
+      rewrite Hmem in *.
+      specialize (Hf a (List.in_eq a xs)).
+      specialize (Ha (eval_iterm a theta)).
+      assert (k = eval_iterm a theta).
+        apply Ha.
+        assert (He := term_dom_valid ds theta Hds a).
+        unfold sat_dom in He; unfold range_of_dom; destruct (term_dom ds a); intuition.
+      congruence.
+    -  apply IHxs; try assumption.
+       inversion Hf; assumption.
+Qed.
+
+Definition notmem_unsat_rec ds z xs :=
+  let (z_db, z_holes) := term_dom ds z in
+  match z_db with
+  | (Bounded l, Bounded u) => zset.zset_covers (notmem_holes ds xs z_holes) l u
+  | _ => false
+  end.
+
+Definition check_notmem_unsat nmem ds :=
+  match nmem with
+      | Notmem z xs =>
+        notmem_unsat_rec ds z xs
+  end.
+Lemma check_notmem_unsat_valid :
+  forall nmem ds, check_notmem_unsat nmem ds = true ->
+                  forall theta, eval_domset ds theta -> ~ eval_notmember nmem theta.
+Proof.
+  intros nmem ds; destruct nmem as [z xs].
+  unfold check_notmem_unsat, notmem_unsat_rec, eval_notmember.
+  eqelim (term_dom ds z).
+  destruct d; destruct b, b0; try (intros; congruence).
+  intros Hcov.
+  rewrite zset.zset_covers_spec in Hcov.
+  intros theta Hds.
+  assert (Hhole := notmem_holes_holes ds theta Hds xs z0).
+  list_ext. intro.
+  assert (Hdom := term_dom_valid ds theta Hds z).
+  specialize (Hhole (eval_iterm z theta)).
+  specialize (Hcov (eval_iterm z theta)).
+  unfold sat_dom in Hdom; rewrite H0 in Hdom; destruct Hdom as [Hb Hh]; simpl in Hb, Hh.
+  unfold sat_dbound, sat_lb, sat_ub in Hb; simpl in Hb.
+  rewrite <- List.Forall_forall in H.
+  assert (~ zset.mem (notmem_holes ds xs z0) (eval_iterm z theta)) as Hnm.
+    apply Hhole; try assumption.
+    refine (List.Forall_impl _ _ H); intuition.
+  specialize (Hcov Hb); contradiction.
+Qed.
+
+Definition MembConstraint : Constraint :=
+  mkConstraint (member) (eval_member).
+Definition MembSolCheck := mkSolChecker MembConstraint check_member_sol check_member_sol_valid.
+Definition MembCheck := mkUnsatChecker MembConstraint check_member_unsat check_member_unsat_valid.
+
+Definition NotmemConstraint : Constraint :=
+  mkConstraint (notmember) (eval_notmember).
+Definition NotmemSolCheck := mkSolChecker NotmemConstraint check_notmem_sol check_notmem_sol_valid.
+Definition NotmemCheck := mkUnsatChecker NotmemConstraint check_notmem_unsat check_notmem_unsat_valid.
